\documentclass[paper=a4, fontsize=11pt]{scrartcl}
\usepackage{fullpage}
\usepackage{amsmath, amsthm, amssymb}
\usepackage[all]{xy}

\usepackage{graphicx}
\usepackage{caption}
\usepackage{subcaption}

\usepackage{xcolor}
\definecolor{bl}{rgb}{0.0,0.2,0.6}
\usepackage{sectsty}
%\usepackage[compact]{titlesec}
\allsectionsfont{\color{bl}\scshape\selectfont}


\begin{document}

\title{\color{bl} Deconvolution by Total Variation Regularization and Iterative Gradient Descent Method}
\author{Yingying Gu}
\date{June 15, 2016}
\maketitle

\section{Deblurring and Denoising by Total Variation Regularization}
Blurry and Gaussian Noisy Image:
\begin{equation}
y=k \ast u + n = Ku + n
\end{equation}
\begin{equation}
u^* \in \underset{u}{\arg\min} ||y-Ku||^2 + \lambda J(u)
\end{equation}
\begin{equation}
E(u) = \lambda \int ||y-k*u||^2 + J(u)
\end{equation}
Total Variation Regularization:
\begin{equation}
J(u)= \sum ||\nabla u||
\end{equation}
or
\begin{equation}
J(u)= \sum \sqrt{||\nabla u||^2+\epsilon}
\end{equation}


\section{Solver: Iterative Gradient Descent Method}
Gradient Descent:
\begin{equation}
u^{(i+1)}= u^{(i)}-\tau \left(k \ast (k \ast u^{(i)}-y)+\lambda Grad J(u^{(i)})\right)
\end{equation}
Where,
\begin{itemize}
  \item The step size $\tau$ can be estimated by line search.
  \item The gradient of the TV term is:
\begin{equation}
Grad J(u)=-div \left(\frac{\nabla u}{\sqrt{||\nabla u||^2+\epsilon}}\right)
\end{equation}
\begin{itemize}
  \item The gradient of u can be computed as
\begin{equation}
\nabla u = [u_x, u_y]
\end{equation}
\begin{equation*}
u_x=u_{i+1,j}-u_{i,j}
\end{equation*}
\begin{equation*}
u_y=u_{i,j+1}-u_{i,j}
\end{equation*}
  \item Euclidean Norm:
\begin{equation}
||\nabla u ||=\sqrt{u_x^2+u_y^2}
\end{equation}
  \item The divergence of the field is the following scheme:
\begin{equation}
div(u)=\frac{\partial u_x}{\partial x}+\frac{\partial u_y}{\partial y}
\end{equation}
\begin{equation*}
(div(u))_{i,j}=
\left\{
  \begin{array}{ll}
    u_x(i,j)-u_x(i-1,j), & \hbox{if 1$<$i$<$n;} \\
    u_x(i,j), & \hbox{if i=1;} \\
    -u_x(i-1,j), & \hbox{if i=n.}
  \end{array}
\right.
\end{equation*}
\begin{equation*}
+
\left\{
  \begin{array}{ll}
    u_y(i,j)-u_y(i,j-1), & \hbox{if 1$<$j$<$n;} \\
    u_y(i,j), & \hbox{if j=1;} \\
    -u_y(i,j-1), & \hbox{if j=n.}
  \end{array}
\right.
\end{equation*}
\end{itemize}
\end{itemize}

\section{Convergence}
\begin{equation}
E(u) = \lambda \int ||y-k*u||^2 + J(u)
\end{equation}
\begin{equation}
|E(u^{i+1})-E(u^{i})| < \epsilon
\end{equation}


\end{document} 